ref_impl/src/verifier/experiments/fstar_experiments/project/testing.fst
@@ -20,8 +20,10 @@ let testa4 = subtypeOf (BTypeUnion BTypeInt BTypeBool) (BTypeUnion BTypeBool BTy
 let testb0 = BTuple 2 (SCons (BInt 342) (SCons (BBool true) (SNil)))
 // The following fails, as expected
 // let test0a1 = BTuple 3 (SCons (BInt 342) (SCons (BBool true) (SNil)))
-let testb1 = BTuple 0 (SNil)
-let testb2 = isTuple 2 (BTypeTuple false 0 (BTypeEmptyTuple)) testb0
+let testb1 = BTuple 0 SNil
+let testb2 = isTuple 0 SNil testb0
+// The following fails, as expected
+// let testb2_ = isTuple 1 SNil testb0
 // let testb3 = isTuple 3 testb0
 // let testb4 = isTuple 2 (BInt 234)
 let testb5 = nthTuple 0 2 testb0
@@ -99,10 +101,9 @@ let _ = assert (forall x y. extractBool (greaterOrEq (max (BInt x) (BInt y)) (BI
 // && (extractBool (eqTerm (max (BInt x) (BBool z)) (BInt x)))
 // )
 
-// val maxWithTuple : x:bosqueTerm{isTuple 2 x} -> y:bosqueTerm{isInt y} -> z:bosqueTerm{isInt z}
-// let maxWithTuple x y = if (extractBool (greaterOrEq (nthTuple 0 2 x) y)) then (nthTuple 0 2 x) else y
-
-val maxWithTuple : x:bosqueTerm{isTuple 2 x} -> y:bosqueTerm{isInt y} -> bosqueTerm
+val maxWithTuple : x:bosqueTerm{isTuple 2 (SCons (BTypeInt) (SCons (BTypeBool) SNil)) x} 
+  -> y:bosqueTerm{isInt y} 
+  -> z:bosqueTerm{isInt z}
 let maxWithTuple x y = let xAt0 = nthTuple 0 2 x in match xAt0 with 
 | BInt x1 -> if (extractBool (greaterOrEq xAt0 y)) then xAt0 else y
 | _ -> BError
@@ -111,10 +112,9 @@ let maxWithTuple x y = let xAt0 = nthTuple 0 2 x in match xAt0 with
 let test4a = maxWithTuple (testb0) (BInt 1203)
 let test4b = maxWithTuple (testb0) (BInt (-12))
 
-// The following fails, as expected
-// let _ = assert (forall x y . extractBool (greaterOrEq (maxWithTuple x y) (nthTuple 0 2 x)))
+let _ = assert (forall x y . extractBool (greaterOrEq (maxWithTuple x y) (nthTuple 0 2 x)))
 
-let _ = assert (forall x y . (bosqueEqType (getType (nthTuple 0 2 x)) (BTypeInt)) ==> extractBool (greaterOrEq (maxWithTuple x y) (nthTuple 0 2 x)))
+let _ = assert (forall x y . (eqType (getType (nthTuple 0 2 x)) BTypeInt) ==> extractBool (greaterOrEq (maxWithTuple x y) (nthTuple 0 2 x)))
 
 (* ---------------------------------------------------------------- *)
 
